test/boot.sh
@@ -43,7 +43,7 @@ check_order alice \
 
 check_order fs \
   "fs: ready, 20 files on the SD card" \
-  "fs: checked: 20 files in 1 folder, 6720 KiB free of 6968, journal 128 KiB"
+  "fs: checked: 20 files in 1 folder, 6716 KiB free of 6968, journal 128 KiB"
 
 check_order mallory \
   "mallory: I am task 2" \
